

# Question 1.

## (a).

The first order derivatives of f with respect to x is:
$$
2a_1y^2x+a_4y+a_5
$$
The second order derivatives of f with respect to x is:
$$
2a_1y^2
$$
The first order derivatives of f with respect to y is:
$$
2a_1x^2y+a_4x
$$
The second order derivatives of f with respect to y is:
$$
2a_1x^2
$$

## (b).

The first order derivatives of f with respect to x is:
$$
2a_1y^2x+2a_2yx+a_3y^2+a_4y+a_5
$$
The second order derivatives of f with respect to x is:
$$
2a_1y^2+2a_2y
$$
The first order derivatives of f with respect to y is:
$$
2a_1x^2y+a_2x^2+2a_3xy+a_4x+a_6
$$
The second order derivatives of f with respect to y is:
$$
2a_1x^2+2a_3x
$$


## (c).

$$
\sigma^`(x)=\frac{e^{-x}}{(1+e^{-x})^2}\\
\sigma(x)=\frac{1}{(1+e^{-x})}\\
(1-\sigma(x))=\frac{1+e^{-x}-1}{(1+e^{-x})}=\frac{e^{-x}}{(1+e^{-x})}\\
So\ \sigma^`(x)=\sigma(x)(1-\sigma(x))
$$



## (d). 

$$
y_1^`=8x-3\\y_1^{``}=8\\
So\ it\ does\ not\ having\ local\ maximum\ points\ and\ the\ minimum\ points\ is \frac{3}{8}.
$$

$$
y_2^`=12x^3-6x^2\\y_2^{``}=36x^2-12x\\
So\ it\ does\ not\ having\ local\ maximum\ points\ and\ the\ minimum\ points.
$$

$$
y_3^`=4+\frac{1}{2\sqrt{1-x}}\\
y_3^{``}=\frac{1}{4\sqrt{(1-x)^3}}\\
So\ it\ does\ not\ having\ local\ maximum\ points\ and\ the\ minimum\ points.
$$

$$
y_4^`=1-\frac{1}{x^2}\\
y_3^{``}=\frac{2}{x^3}\\
So\ it\ has\ local\ maximum\ points\ of\ -1\  and\ the\ minimum\ points\ of \ 1.
$$



# Question 2.

## (a).

$$
P(A)=\frac{20\%+10\%}{1}=0.3\\
P(B)=\frac{(1-20\%10\%-40\%)+10\%}{1}=0.4\\
P(A \cup B)=\frac{10\%}{1}=0.1\\
P(A)=\frac{40\%}{1}=0.4\\
$$

## (b).

(i).
$$
r=1-\frac{1}{6}-\frac{1}{12}-\frac{1}{12}-\frac{1}{6}-\frac{1}{6}=\frac{1}{3}
$$
(ii).
$$
P(X=2,Y=3)=\frac{1}{6}
$$
(iii).
$$
P(X=3)=0+r+0=0+\frac{1}{3}+0=\frac{1}{3}\\
P(X=3,Y=2)=r=\frac{1}{3}
$$


(iv).
$$
E(X)=1*\frac{1}{3}+2*\frac{1}{3}+3*\frac{1}{3}=2\\
E(Y)=1*\frac{1}{3}+2*\frac{5}{12}+3*\frac{3}{12}=\frac{23}{12}\\
E(XY)=1*\frac{1}{6}+2*\frac{1}{12}+3*\frac{1}{12}+2*\frac{1}{6}+4*0+6*\frac{1}{6}+3*0+6*\frac{1}{3}+9*0=\frac{47}{12}
$$


(v).
$$
E(X^2)=1*\frac{1}{3}+4*\frac{1}{3}+9*\frac{1}{3}=\frac{14}{3}\\
E(Y^2)=1*\frac{1}{3}+4*\frac{5}{12}+9*\frac{3}{12}=\frac{17}{4}\\
$$


(vi).
$$
Cov(X,Y)=E(XY)-E(X)*E(Y)=\frac{47}{12}-2*\frac{9}{4}=-\frac{7}{12}
$$


(vii).
$$
Var(X)=E(X^2)-{E(X)}^2=\frac{14}{3}-2*2=\frac{2}{3}\\
Var(Y)=E(Y^2)-{E(Y)}^2=\frac{17}{4}-\frac{23}{12}*\frac{23}{12}=\frac{83}{144}
$$


(viii).
$$
Corr(X,Y)=\frac{Cov(X,Y)}{\sqrt{Var{X}}*\sqrt{Var(Y)}}=-\frac{7\sqrt{3}}{\sqrt{166}}
$$




# Question3.

(a).

The dimensions of A is 3 * 5, the dimention of B is 6 * 1, the dimension of A^T is 5 * 3.



(b).

(i). AB and BA is not exists.

(ii)
$$
AC=\\
[21,14,14\\20,10,10\\56,28,28]\\
CA=\\
[31,39,40\\10,12,12\\18,18,16]
$$
(iii).
$$
AD=\\
[20,32\\
17,19\\
43,45]
$$
DA is not exist.



(iv).

DC is not exist.
$$
CD=\\
[43,41\\11,13\\18,22]\\
D^TC=\\
[38,18,18\\32,18,18]
$$


(v).
$$
Bu=\\
[14\\4]
$$
uB is not exist.



(vi).

Au is not exist.



(vii).
$$
Av=\\
[18\\13\\31]
$$
vA is not exist.



(viii).
$$
Av+Cv=\\
[47\\22\\45]
$$


(c).

(i).
$$
{||u||}_1=|1|+|3|=4\\
{||u||}_2=\sqrt{1^2+3^2}=\sqrt{10}\\
{||u||}_2^2=1^2+3^2=10\\
{||u||}_\infty=3\\
$$
(ii).
$$
{||u||}_1=|2|+|4|+|1|=7\\
{||u||}_2=\sqrt{2^2+4^2+1^2}=\sqrt{21}\\
{||u||}_2^2=2^2+4^2+1^2=21\\
{||u||}_\infty=4\\
$$


(iii).
$$
v+w=\\
[3\\2\\3]\\
{||v+w||}_1=|3|+|2|+|3|=8\\
{||v+w||}_2=\sqrt{3^2+2^2+3^2}=\sqrt{22}\\
{||v+w||}_2^2=3^2+2^2+3^2=22\\
{||v+w||}_\infty=3\\
$$


(iv).
$$
Av=\\
[18\\13\\31]\\
A(v-w)=\\
[15\\13\\27]\\
{||Av||}_2=\sqrt{18^2+13^2+31^2}=\sqrt{1454}\\
{||A(v-w||}_\infty=27\\
$$
(d).
$$
<u,v>=3\\
<u,w>=0\\
<v,w>=-\frac{1}{2}\\
$$


(e).

A dot product of 0 proves that the two vectors are orthogonal, a positive dot product indicates that the angle between the two vectors is acute angle, and a negative dot product indicates that the angle between the two vectors is obtuse angle.



(f).

the inverse of A is:
$$
[-\frac{1}{11},\frac{3}{11}\\\frac{4}{11}, -\frac{1}{11}]
$$


(g).

A is a Singular matrix, so it has not the inverse matrix.



(h).
$$
{(X^TX)}^T=X^T{(X^T)}^T=X^TX\\
So\ that\ X^TX\ is\ always\ symmetric.
$$
